Checkpoint paxos resources/invariants

src/program_proof/tulip/paxos/base.v
@@ -9,7 +9,7 @@ Inductive nodedec :=
 | Accept (v : ledger)
 | Reject.
 
-Definition ballot := list nodedec.
+Definition ballot := gmap nat nodedec.
 
 Section def.
   Context `{Countable A}.
@@ -41,25 +41,23 @@ Section def.
     prefix v1 v2.
 
   (* Compute the latest term in which a proposal is accepted before [n]. *)
-  Fixpoint latest_term_before t l : nat :=
+  Fixpoint latest_term_before `{Lookup nat nodedec B} t (m : B) :=
     match t with
     | O => O
-    | S p => match l !! p with
+    | S p => match m !! p with
             | Some d => match d with
                        | Accept _ => p
-                       | Reject => latest_term_before p l
+                       | Reject => latest_term_before p m
                        end
-            | _ => latest_term_before p l
+            | _ => latest_term_before p m
             end
     end.
-
-  (* Definition latest_term (l : ballot) := latest_before (length l) l. *)
 
   Definition latest_term_before_quorum_step (x : A) (cur prev : nat) : nat :=
     cur `max` prev.
 
-  Definition latest_term_before_quorum bsq t :=
-    let ts := fmap (latest_term_before t) bsq in
+  Definition latest_term_before_quorum `{Lookup nat nodedec B} (ms : gmap A B) t :=
+    let ts := fmap (latest_term_before t) ms in
     map_fold latest_term_before_quorum_step O ts.
 
   Definition longest_proposal_step (x : A) (cur prev : option ledger) :=
@@ -76,25 +74,28 @@ Section def.
   Definition longest_proposal ovs :=
     map_fold longest_proposal_step None ovs.
 
-  Definition longest_proposal_in_term bsq t :=
-    let ovs := fmap (λ l, match l !! t with
-                          | Some (Accept v) => Some v
-                          | _ => None
-                          end) bsq in
+  Definition ledger_at_term `{Lookup nat nodedec B} t (m : B) :=
+    match m !! t with
+    | Some (Accept v) => Some v
+    | _ => None
+    end.
+
+  Definition longest_proposal_in_term `{Lookup nat nodedec B} (ms : gmap A B) t :=
+    let ovs := fmap (ledger_at_term t) ms in
     longest_proposal ovs.
 
-  Definition equal_latest_longest_proposal bsq psb t v :=
-    let t' := latest_term_before_quorum bsq t in
-    longest_proposal_in_term bsq t' = Some v.
+  Definition equal_latest_longest_proposal `{Lookup nat nodedec B} (ms : gmap A B) t v :=
+    let t' := latest_term_before_quorum ms t in
+    longest_proposal_in_term ms t' = Some v.
 
-  Definition valid_base_proposal bs psb t v :=
+  Definition valid_base_proposal bs t v :=
     ∃ bsq : gmap A ballot,
       bsq ⊆ bs ∧
       cquorum_size (dom bs) (dom bsq) ∧
-      equal_latest_longest_proposal bsq psb t v.
+      equal_latest_longest_proposal bsq t v.
 
   Definition valid_base_proposals bs psb :=
-    map_Forall (λ n v, valid_base_proposal bs psb n v) psb.
+    map_Forall (λ n v, valid_base_proposal bs n v) psb.
 
   Definition valid_lb_ballot psb l :=
     ∀ t v, l !! t = Some (Accept v) -> ∃ v', psb !! t = Some v' ∧ prefix v' v.
@@ -111,7 +112,31 @@ Section def.
   Definition valid_proposals ps psb :=
     map_Forall2 (λ _ (lb l : ledger), prefix lb l) psb ps.
 
+  Definition free_term_with_partf (P : A -> nat -> Prop) (ts : gset nat) (x : A) (t : nat) :=
+    ∀ t', P x t' -> (t < t')%nat -> t' ∉ ts.
+
+  Definition free_terms_with_partf (P : A -> nat -> Prop) (ts : gset nat) (tm : gmap A nat) :=
+    (∀ x1 x2 t, x1 ≠ x2 -> P x1 t -> not (P x2 t)) ∧
+    map_Forall (λ x n, free_term_with_partf P ts x n) tm.
+
 End def.
+
+Definition max_nodes : Z := 16.
+
+Definition is_term_of_node (x : u64) (t : nat) :=
+  t `mod` max_nodes = (uint.Z x).
+
+Lemma is_term_of_node_partitioned x1 x2 t :
+  x1 ≠ x2 -> is_term_of_node x1 t -> not (is_term_of_node x2 t).
+Proof.
+  unfold is_term_of_node.
+  intros Hne Hx1.
+  rewrite Hx1.
+  by apply word.unsigned_inj'.
+Qed.
+
+Definition free_terms ts tm :=
+  free_terms_with_partf is_term_of_node ts tm.
 
 Class paxos_ghostG (Σ : gFunctors).
 
