src/program_proof/tulip/paxos/res.v
@@ -1,0 +1,450 @@
+From Perennial.program_proof Require Import grove_prelude.
+From Perennial.program_proof.rsm.pure Require Import quorum.
+From Perennial.program_proof.tulip.paxos Require Import base.
+
+Section res.
+  Context `{!paxos_ghostG Σ}.
+  (* TODO: remove this once we have real defintions for resources. *)
+  Implicit Type (γ : paxos_names).
+
+  Section consensus.
+
+    (** Elements. *)
+
+    Definition own_log_half γ (l : ledger) : iProp Σ.
+    Admitted.
+
+    Definition is_log_lb γ (l : ledger) : iProp Σ.
+    Admitted.
+
+    Definition own_cpool_half γ (vs : gset string) : iProp Σ.
+    Admitted.
+
+    (** Type class instances. *)
+
+    #[global]
+    Instance is_log_lb_persistent γ l :
+      Persistent (is_log_lb γ l).
+    Admitted.
+
+    (** Rules. *)
+
+    Lemma log_update {γ} l1 l2 vs :
+      Forall (λ v, v ∈ vs) l2 ->
+      prefix l1 l2 ->
+      own_log_half γ l1 -∗
+      own_log_half γ l1 -∗
+      own_cpool_half γ vs ==∗
+      own_log_half γ l2 ∗ own_log_half γ l2 ∗ own_cpool_half γ vs.
+    Admitted.
+
+    Lemma log_witness {γ l} :
+      own_log_half γ l -∗
+      is_log_lb γ l.
+    Admitted.
+
+    Lemma log_prefix {γ l lb} :
+      own_log_half γ l -∗
+      is_log_lb γ lb -∗
+      ⌜prefix lb l⌝.
+    Admitted.
+
+    Lemma log_lb_prefix {γ lb1 lb2} :
+      is_log_lb γ lb1 -∗
+      is_log_lb γ lb2 -∗
+      ⌜prefix lb1 lb2 ∨ prefix lb2 lb1⌝.
+    Admitted.
+
+    Lemma cpool_update {γ vs1} vs2 :
+      vs1 ⊆ vs2 ->
+      own_cpool_half γ vs1 -∗
+      own_cpool_half γ vs1 ==∗
+      own_cpool_half γ vs2 ∗ own_cpool_half γ vs2.
+    Admitted.
+
+    Definition cpool_subsume_log (l : ledger) (vs : gset string) :=
+      Forall (λ v, v ∈ vs) l.
+
+    Lemma consensus_incl {γ l vs} :
+      own_log_half γ l -∗
+      own_cpool_half γ vs -∗
+      ⌜cpool_subsume_log l vs⌝.
+    Admitted.
+
+  End consensus.
+
+  Section internal_log.
+
+    (** Elements. *)
+
+    Definition own_internal_log γ (l : ledger) : iProp Σ.
+    Admitted.
+
+    Definition is_internal_log_lb γ (l : ledger) : iProp Σ.
+    Admitted.
+
+    (** Type class instances. *)
+
+    #[global]
+    Instance is_internal_log_lb_persistent γ l :
+      Persistent (is_internal_log_lb γ l).
+    Admitted.
+
+    (** Rules. *)
+
+    Lemma internal_log_update {γ l1} l2 :
+      prefix l1 l2 ->
+      own_internal_log γ l1 ==∗
+      own_internal_log γ l2.
+    Admitted.
+
+    Lemma internal_log_witness {γ l} :
+      own_internal_log γ l -∗
+      is_internal_log_lb γ l.
+    Admitted.
+
+    Lemma internal_log_prefix {γ l lb} :
+      own_internal_log γ l -∗
+      is_internal_log_lb γ lb -∗
+      ⌜prefix lb l⌝.
+    Admitted.
+
+  End internal_log.
+
+  Section proposal.
+
+    (** Elements. *)
+
+    Definition own_proposals γ (vs : proposals) : iProp Σ.
+    Admitted.
+
+    Definition own_proposal γ (t : nat) (v : ledger) : iProp Σ.
+    Admitted.
+
+    Definition is_proposal_lb γ (t : nat) (v : ledger) : iProp Σ.
+    Admitted.
+
+    (** Type class instances. *)
+
+    #[global]
+    Instance is_proposal_lb_persistent γ t v :
+      Persistent (is_proposal_lb γ t v).
+    Admitted.
+
+    (** Rules. *)
+
+    Lemma proposal_insert {γ vs} t v :
+      vs !! t = None ->
+      own_proposals γ vs ==∗
+      own_proposals γ (<[t := v]> vs) ∗ own_proposal γ t v.
+    Admitted.
+
+    Lemma proposal_lookup {γ vs t v} :
+      own_proposal γ t v -∗
+      own_proposals γ vs -∗
+      ⌜vs !! t = Some v⌝.
+    Admitted.
+
+    Lemma proposal_update {γ vs t v1} v2 :
+      prefix v1 v2 ->
+      own_proposal γ t v1 -∗
+      own_proposals γ vs ==∗
+      own_proposal γ t v2 ∗ own_proposals γ (<[t := v2]> vs).
+    Admitted.
+
+    Lemma proposal_witness {γ t v} :
+      own_proposal γ t v -∗
+      is_proposal_lb γ t v.
+    Admitted.
+
+    Lemma proposal_prefix {γ t vlb v} :
+      is_proposal_lb γ t vlb -∗
+      own_proposal γ t v -∗
+      ⌜prefix vlb v⌝.
+    Admitted.
+
+  End proposal.
+
+  Section base_proposal.
+
+    (** Elements. *)
+
+    Definition own_base_proposals γ (vs : proposals) : iProp Σ.
+    Admitted.
+
+    Definition is_base_proposal_receipt γ (t : nat) (v : ledger) : iProp Σ.
+    Admitted.
+
+    (** Type class instances. *)
+
+    #[global]
+    Instance is_base_proposal_receipt_persistent γ t v :
+      Persistent (is_base_proposal_receipt γ t v).
+    Admitted.
+
+    (** Rules. *)
+
+    Lemma base_proposal_insert {γ vs} t v :
+      vs !! t = None ->
+      own_base_proposals γ vs ==∗
+      own_base_proposals γ (<[t := v]> vs) ∗ is_base_proposal_receipt γ t v.
+    Admitted.
+
+    Lemma base_proposal_lookup {γ vs t v} :
+      is_base_proposal_receipt γ t v -∗
+      own_base_proposals γ vs -∗
+      ⌜vs !! t = Some v⌝.
+    Admitted.
+
+  End base_proposal.
+
+  Section past_nodedecs.
+
+    (** Elements. *)
+
+    Definition own_past_nodedecs γ (nid : u64) (d : list nodedec) : iProp Σ.
+    Admitted.
+
+    Definition is_past_nodedecs_lb γ (nid : u64) (d : list nodedec) : iProp Σ.
+    Admitted.
+
+    (** Type class instances. *)
+
+    #[global]
+    Instance is_past_nodedecs_lb_persistent γ nid d :
+      Persistent (is_past_nodedecs_lb γ nid d).
+    Admitted.
+
+    (** Rules. *)
+
+    Lemma past_nodedecs_update γ nid d1 d2 :
+      prefix d1 d2 ->
+      own_past_nodedecs γ nid d1 ==∗
+      own_past_nodedecs γ nid d2.
+    Admitted.
+
+    Lemma past_nodedecs_witness γ nid d :
+      own_past_nodedecs γ nid d -∗
+      is_past_nodedecs_lb γ nid d.
+    Admitted.
+
+    Lemma past_nodedecs_prefix γ nid dlb d :
+      is_past_nodedecs_lb γ nid dlb -∗
+      own_past_nodedecs γ nid d -∗
+      ⌜prefix dlb d⌝.
+    Admitted.
+
+  End past_nodedecs.
+
+  Section accepted_proposal.
+
+    (** Elements. *)
+
+    Definition own_accepted_proposals γ (nid : u64) (vs : proposals) : iProp Σ.
+    Admitted.
+
+    Definition own_accepted_proposal γ (nid : u64) (t : nat) (v : ledger) : iProp Σ.
+    Admitted.
+
+    Definition is_accepted_proposal_lb γ (nid : u64) (t : nat) (v : ledger) : iProp Σ.
+    Admitted.
+
+    (** Type class instances. *)
+
+    #[global]
+    Instance is_accepted_proposal_lb_persistent γ nid t v :
+      Persistent (is_accepted_proposal_lb γ nid t v).
+    Admitted.
+
+    (** Rules. *)
+
+    Lemma accepted_proposal_insert {γ nid vs t v} :
+      vs !! t = None ->
+      own_accepted_proposals γ nid vs ==∗
+      own_accepted_proposals γ nid (<[t := v]> vs) ∗ own_accepted_proposal γ nid t v.
+    Admitted.
+
+    Lemma accepted_proposal_update {γ nid vs t v1} v2 :
+      prefix v1 v2 ->
+      own_accepted_proposal γ nid t v1 -∗
+      own_accepted_proposals γ nid vs ==∗
+      own_accepted_proposal γ nid t v2 ∗ own_accepted_proposals γ t (<[t := v2]> vs).
+    Admitted.
+
+  End accepted_proposal.
+
+  Section current_term.
+
+    (** Elements. *)
+
+    Definition own_current_term_half γ (nid : u64) (t : nat) : iProp Σ.
+    Admitted.
+
+    (** Type class instances. *)
+
+    (** Rules. *)
+
+    Lemma current_term_update {γ nid t1} t2 :
+      own_current_term_half γ nid t1 -∗
+      own_current_term_half γ nid t1 ==∗
+      own_current_term_half γ nid t2 ∗ own_current_term_half γ nid t2.
+    Admitted.
+
+    Lemma current_term_agree {γ nid t1 t2} :
+      own_current_term_half γ nid t1 -∗
+      own_current_term_half γ nid t2 -∗
+      ⌜t2 = t1⌝.
+    Admitted.
+
+  End current_term.
+
+  Section ledger_term.
+
+    (** Elements. *)
+
+    Definition own_ledger_term_half γ (nid : u64) (t : nat) : iProp Σ.
+    Admitted.
+
+    (** Type class instances. *)
+
+    (** Rules. *)
+
+    Lemma ledger_term_update {γ nid t1} t2 :
+      own_ledger_term_half γ nid t1 -∗
+      own_ledger_term_half γ nid t1 ==∗
+      own_ledger_term_half γ nid t2 ∗ own_ledger_term_half γ nid t2.
+    Admitted.
+
+    Lemma ledger_term_agree {γ nid t1 t2} :
+      own_ledger_term_half γ nid t1 -∗
+      own_ledger_term_half γ nid t2 -∗
+      ⌜t2 = t1⌝.
+    Admitted.
+
+  End ledger_term.
+
+  Section node_ledger.
+
+    (** Elements. *)
+
+    Definition own_node_ledger_half γ (nid : u64) (v : ledger) : iProp Σ.
+    Admitted.
+
+    (** Type class instances. *)
+
+    (** Rules. *)
+
+    Lemma node_ledger_update {γ nid v1} v2 :
+      own_node_ledger_half γ nid v1 -∗
+      own_node_ledger_half γ nid v1 ==∗
+      own_node_ledger_half γ nid v2 ∗ own_node_ledger_half γ nid v2.
+    Admitted.
+
+    Lemma node_ledger_agree {γ nid v1 v2} :
+      own_node_ledger_half γ nid v1 -∗
+      own_node_ledger_half γ nid v2 -∗
+      ⌜v2 = v1⌝.
+    Admitted.
+
+  End node_ledger.
+
+End res.
+
+Section inv.
+  Context `{!heapGS Σ, !paxos_ghostG Σ}.
+
+  Definition paxosNS := nroot .@ "paxos".
+
+  Definition fixed_proposals (ds : list nodedec) (ps : proposals) :=
+    ∀ t od, ds !! t = od ->
+            match od with
+            | Some (Accept v) => ps !! t = Some v
+            | Some Reject => ps !! t = None
+            | _ => True
+            end.
+
+  Definition free_terms_after (t : nat) (ts : gset nat) :=
+    ∀ t', (t < t')%nat -> t' ∉ ts.
+
+
+  Definition node_inv γ nid terml : iProp Σ :=
+    ∃ ds psa termc logn,
+      "Hblt"   ∷ own_past_nodedecs γ nid ds ∗
+      "Hpsa"   ∷ own_accepted_proposals γ nid psa ∗
+      "Htermc" ∷ own_current_term_half γ nid termc ∗
+      "Hterml" ∷ own_ledger_term_half γ nid terml ∗
+      "Hlogn"  ∷ own_node_ledger_half γ nid logn ∗
+      "%Hfixed"  ∷ ⌜fixed_proposals ds psa⌝ ∗
+      "%Hdompsa" ∷ ⌜free_terms_after terml (dom psa)⌝ ∗
+      "%Hlogn"   ∷ ⌜psa !! terml = Some logn⌝ ∗
+      "%Hlenblt" ∷ ⌜length ds = termc⌝ ∗
+      "%Htermlc" ∷ ⌜(terml ≤ termc)%nat⌝ ∗
+      "%Hlatest" ∷ ⌜terml ≠ termc -> latest_term_before termc ds = terml⌝.
+
+  Definition prefix_of_accepted_proposal γ nid t logi: iProp Σ :=
+    ∃ loga,
+      "#Hloga"   ∷ is_accepted_proposal_lb γ nid t loga ∗
+      "%Hprefix" ∷ ⌜prefix logi loga⌝.
+
+  Definition safe_internal_log γ nids logi : iProp Σ :=
+    ∃ nidsq t,
+      "#Hacpt"   ∷ ([∗ set] nid ∈ nidsq, prefix_of_accepted_proposal γ nid t logi) ∗
+      "%Hquorum" ∷ ⌜cquorum_size nids nidsq⌝.
+
+  Definition safe_base_proposal γ nids t v : iProp Σ :=
+    ∃ dsq,
+      "#Hdsq"    ∷ ([∗ map] nid ↦ d ∈ dsq, is_past_nodedecs_lb γ nid d) ∗
+      "%Hlen"    ∷ ⌜map_Forall (λ _ d, (t ≤ length d)%nat) dsq⌝ ∗
+      "%Hincl"   ∷ ⌜dom dsq ⊆ nids⌝ ∗
+      "%Hquorum" ∷ ⌜cquorum_size nids (dom dsq)⌝ ∗
+      "%Heq"     ∷ ⌜equal_latest_longest_proposal dsq t v⌝.
+
+  Definition paxos_inv γ nids : iProp Σ :=
+    ∃ log cpool logi ps psb termlm,
+      (* external states *)
+      "Hlog"   ∷ own_log_half γ log ∗
+      "Hcpool" ∷ own_cpool_half γ cpool ∗
+      (* internal states *)
+      "Hlogi" ∷ own_internal_log γ logi ∗
+      "Hps"   ∷ own_proposals γ ps ∗
+      "Hpsb"  ∷ own_base_proposals γ psb ∗
+      (* node states *)
+      "Hnodes" ∷ ([∗ map] nid ↦ terml ∈ termlm, node_inv γ nid terml) ∗
+      (* TODO: constraints between internal and external states *)
+      (* constraints on internal states *)
+      "#Hsafelogi" ∷ safe_internal_log γ nids logi ∗
+      "#Hsafepsb"  ∷ ([∗ map] t ↦ v ∈ psb, safe_base_proposal γ nids t v) ∗
+      "%Hbase"     ∷ ⌜map_Forall2 (λ _ (vlb v : ledger), prefix vlb v) psb ps⌝ ∗
+      "%Hdompsb"   ∷ ⌜free_terms (dom psb) termlm⌝.
+
+  #[global]
+  Instance paxos_inv_timeless γ nids :
+    Timeless (paxos_inv γ nids).
+  Admitted.
+
+  Definition know_paxos_inv γ nids : iProp Σ :=
+    inv paxosNS (paxos_inv γ nids).
+
+End inv.
+
+(**
+ * Notes on state-machine actions of Paxos:
+ * - nominate(termc)
+ * - ascend(t, v): insert [(t, v)] into [proposals] and [base_proposals].
+ * - extend(t, v): update [proposals !! t] to [v]
+ * - prepare(t): snoc [accepted_proposals !! (length ballot)] to [ballot] if it exists, and extend [ballot] with [Reject] up to [t].
+ * - accept(t, v): same as prepare(t), but additionally insert/update [(t, v)] to [accepted_proposals].
+ * - commit(v): update [internal_log] to [v].
+ *)
+
+Section invariance.
+  Context `{!paxos_ghostG Σ}.
+
+  Lemma paxos_inv_nominate γ nids nid termc termc' :
+    own_current_term_half γ nid termc -∗
+    paxos_inv γ nids ==∗
+    own_current_term_half γ nid termc' ∗
+    paxos_inv γ nids.
+  Admitted.
+
+End invariance.
